src/examples/Kuiper.Sparse.Array.Iterator.fst
@@ -1,0 +1,139 @@
+module Kuiper.Sparse.Array.Iterator
+
+#lang-pulse
+open Kuiper
+open Kuiper.Sparse.Common
+open Kuiper.Sparse.Array
+module SZ = FStar.SizeT
+
+// This is here to force extraction.
+let _ = 1ul
+
+(* iterador sobre array esparso *)
+
+inline_for_extraction
+type sarray_iterator
+  (#et : Type0) (#l : erased nat)
+  (a : sarray et l) =
+{
+  i   : (i   : sz{i <= a.nnz}); // índice en elems
+}
+
+inline_for_extraction noextract
+fn sarray_iterator_init
+  (#et : Type0) {| scalar et |}
+  (#l : erased nat)
+  (a : sarray et l)
+  (#f : perm)
+  (#s : erased (seq et))
+  (#v_elems : erased (seq et){Seq.length v_elems == a.nnz})
+  (#v_pos   : erased (seq sz){Seq.length v_pos   == a.nnz})
+  preserves gpu
+  preserves sarray_pts_to' a #f s v_elems v_pos
+  returns i : sarray_iterator #et #l a
+  ensures pure (
+    forall (j : natlt (Seq.length s)).
+      i.i < a.nnz /\ j < v_pos @! i.i ==> s @! j == zero
+  )
+{
+    let i : sarray_iterator a = { i = 0sz };
+    unfold sarray_pts_to' a #f s v_elems v_pos;
+    fold sarray_pts_to' a #f s v_elems v_pos;
+    i;
+}
+
+inline_for_extraction noextract
+let sarray_iterator_end
+  (#et : Type0) (#l : erased nat)
+  (#a : sarray et l)
+  (i : sarray_iterator a)
+  : bool =
+  i.i = a.nnz
+
+inline_for_extraction noextract
+fn sarray_iterator_get
+  (#et : Type0) {| scalar et |}
+  (#l : erased nat)
+  (#a : sarray et l)
+  (#s : erased (seq et))
+  (i : sarray_iterator a)
+  preserves gpu ** a |-> s
+  requires
+    pure (not (sarray_iterator_end i))
+  returns v : sz & et
+{
+  unfold sarray_pts_to a s;
+  with v_elems v_pos.
+    assert sarray_pts_to' a s v_elems v_pos;
+    unfold sarray_pts_to' a s v_elems v_pos;
+
+  let v = gpu_array_read a.elems i.i;
+  let p = gpu_array_read a.pos i.i;
+
+  fold sarray_pts_to' a s v_elems v_pos;
+  fold sarray_pts_to a s;
+  (p, v)
+}
+
+inline_for_extraction noextract
+fn sarray_iterator_next
+  (#et : Type0) {| scalar et |}
+  (#l : erased nat)
+  (#a : sarray et l)
+  (i : sarray_iterator a)
+  (#f : perm)
+  (#s : erased (seq et))
+  (#v_elems : erased (seq et){len v_elems == a.nnz})
+  (#v_pos   : erased (seq sz){len v_pos   == a.nnz})
+  (#_ : squash (not (sarray_iterator_end i)))
+  preserves gpu
+  preserves sarray_pts_to' a #f s v_elems v_pos
+  requires
+    pure (not (sarray_iterator_end i))
+  returns i' : sarray_iterator a
+  ensures pure (
+    forall (j : natlt (len s)).
+    v_pos @! i.i < j /\
+      (if i'.i = a.nnz then true else j < v_pos @! i'.i)
+      ==> s @! j == zero
+  )
+{
+  unfold sarray_pts_to' a #f s v_elems v_pos;
+    let i' : sarray_iterator a = {i = i.i +^ 1sz};
+    fold sarray_pts_to' a #f s v_elems v_pos;
+    i'
+}
+
+inline_for_extraction noextract
+fn sarray_iterator_test
+  (#et : eqtype) {| ets: scalar et |}
+  (#l : erased nat)
+  (a : sarray et l)
+  (#s : erased (seq et))
+  preserves gpu ** a |-> s
+  ensures emp
+{
+  unfold sarray_pts_to a;
+
+  with v_elems v_pos.
+    assert sarray_pts_to' a s v_elems v_pos;
+
+  let mut it : sarray_iterator #et #l a = sarray_iterator_init a;
+
+  fold sarray_pts_to a s;
+
+  while (not (sarray_iterator_end !it))
+    invariant
+      live it
+  {
+    let r = sarray_iterator_get !it;
+
+    unfold sarray_pts_to a s;
+
+    it := sarray_iterator_next #et #ets #l #a !it #1.0R #s;
+
+    fold sarray_pts_to a s;
+  };
+}
+
+let sarray_iterator_test_u32 #l = sarray_iterator_test #u32 #_ #l
