src/examples/Kuiper.Sparse.Array.fst
@@ -1,0 +1,72 @@
+module Kuiper.Sparse.Array
+
+#lang-pulse
+open Kuiper
+open Kuiper.Sparse.Common
+module SZ = FStar.SizeT
+
+// This is here to force extraction.
+let _ = 1ul
+
+(* Sparse array *)
+noextract
+let valid_pos (#nnz l : nat) (s : lseq nat nnz) : prop
+= in_bounds 0 l s /\ sorted s
+
+noeq
+inline_for_extraction
+type sarray (et : Type0)
+  (l : erased nat) =
+  // ^ longitud "virtual" del array
+{ nnz   : sz; // número de no-zeros len   : (len : sz {SZ.v len == reveal l}); // longitud "real" del array virtual
+  elems : gpu_array et nnz; // elementos (no zero)
+  pos   : gpu_array sz nnz; // posición de cada elemento
+}
+
+let unsparse
+  (#et:Type0) {| scalar et |}
+  (nnz l : nat)
+  (elems : lseq et nnz)
+  (pos   : lseq nat nnz{valid_pos l pos})
+  : GTot (lseq et l)
+=
+  let open FStar.Seq in
+  init l fun i ->
+    if mem i pos
+      then elems @! index_mem i pos
+      else zero
+
+let sarray_pts_to'
+  (#et:Type0) {| d : scalar et |} (#l : nat)
+  (a : sarray et l)
+  (#[Tactics.exact (`1.0R)] f : perm)
+  (s : seq et)
+  (v_elems : lseq et a.nnz)
+  (v_pos   : lseq sz a.nnz)
+  : slprop
+=
+    a.elems |-> Frac f v_elems **
+    a.pos   |-> Frac f v_pos **
+    pure (
+      valid_pos l (cast_pos #a.nnz v_pos <: lseq nat a.nnz)
+      /\ s == unsparse a.nnz l v_elems (cast_pos v_pos)
+    )
+
+let sarray_pts_to
+  (#et:Type0) {| d : scalar et |} #l
+  (a : sarray et l)
+  (#[Tactics.exact (`1.0R)] f : perm)
+  (s : seq et)
+  : slprop
+=
+  exists* (v_elems : lseq et a.nnz) (v_pos : lseq sz a.nnz).
+    sarray_pts_to' a #f s v_elems v_pos
+
+inline_for_extraction noextract
+unfold
+instance has_pts_to_sarray
+  (#et: Type0) (#l : nat) {| scalar et |}
+  : has_pts_to (sarray et l) (seq et) =
+{
+  pts_to = sarray_pts_to;
+}
