src/examples/Kuiper.Sparse.Common.fst
@@ -1,0 +1,104 @@
+module Kuiper.Sparse.Common
+
+#lang-pulse
+open Kuiper
+module SZ = FStar.SizeT
+
+// This is here to force extraction.
+let _ = 1ul
+
+(* Propiedades sobre escalares *)
+
+assume
+val zero_is_absorbing_l
+  (#et:_) {| scalar et |}
+  (k : et)
+  : Lemma
+    (requires true)
+    (ensures k `mul` zero == zero)
+    [SMTPat (k `mul` zero)]
+    // FIXME: ^ this pattern does not kick in
+    // if we use `d.mul` instead of `mul`. Why?
+
+assume
+val zero_is_absorbing_r
+  (#et:_) {| scalar et |}
+  (k : et)
+  : Lemma
+    (requires true)
+    (ensures zero `mul` k == zero)
+    [SMTPat (zero `mul` k )]
+
+assume
+val zero_is_id_l
+  (#et:_) {| scalar et |}
+  (k : et)
+  : Lemma
+    (requires true)
+    (ensures k `add` zero == k)
+    [SMTPat (k `add` zero)]
+
+assume
+val zero_is_id_r
+  (#et:_) {| scalar et |}
+  (k : et)
+  : Lemma
+    (requires true)
+    (ensures zero `add` k == k)
+    [SMTPat (zero `add` k)]
+
+(* Secuencias *)
+
+
+let map_seq_len (#a #b:Type) (f:a -> Tot b) (s:Seq.seq a)
+  : Lemma (ensures len (Seq.map_seq f s) == len s)
+          [SMTPat (Seq.map_seq f s)]
+  = Seq.map_seq_len f s
+
+let my_map_seq_index (#a #b:Type) (f:a -> Tot b) (s:Seq.seq a) (i:nat{i < len s})
+  : Lemma (ensures (Seq.map_seq_len f s; Seq.map_seq f s @! i == f (s @! i)))
+          [SMTPat (Seq.map_seq f s @! i)]
+  = Seq.map_seq_index f s i
+
+
+(* Propiedades sobre las posiciones de un array esparso *)
+
+noextract
+let in_bounds (l h : nat) (s : seq nat) : prop =
+  forall i. {:pattern (s @! i)} l <= s @! i /\ s @! i < h
+
+noextract
+let sorted_slice
+  (s : seq nat)
+  (a b : nat{a <= b /\ b <= len s})
+  : prop
+=
+  forall i j. {:pattern (s @! i); (s @! j)} a <= i /\ i < j /\ j < b ==> s @! i < s @! j
+
+
+noextract
+let sorted (s : seq nat) : prop =
+  sorted_slice s 0 (len s)
+
+let rec bounded_from_sorted_in_bounds
+  (#nnz l h : nat)
+  (s : lseq nat nnz)
+  : Lemma
+    (requires l <= h /\ sorted s /\ in_bounds l h s)
+    (ensures nnz + l <= h)
+=
+  let open FStar.Seq in
+
+  if nnz = 0
+    then ()
+    else bounded_from_sorted_in_bounds #(nnz - 1) ((s @! 0) + 1) h (tail s)
+
+let cast_pos
+  (#nnz : nat)
+  (pos : lseq sz nnz)
+  : Ghost
+    (lseq nat nnz)
+    (requires true)
+    (ensures fun npos -> forall i. npos @! i == SZ.v (pos @! i))
+=
+  Seq.map_seq SZ.v pos
